\documentclass[letterpaper]{article}

\usepackage{fullpage}
\usepackage{nopageno}
\usepackage{amsmath}
\usepackage{amssymb}
\usepackage[utf8]{inputenc}
\allowdisplaybreaks

\newcommand{\abs}[1]{\left\lvert #1 \right\rvert}

\begin{document}
\title{Notes}
\date{November 26, 2014}
\maketitle
\section*{section 6.2.4}
let $f:[a,b]\to\mathbb{R}$ be differentiable, then
\begin{enumerate}
\item
if $f'$ is (strictly) positive, $f$ is (strictly) increasing
\item
same for negative
\item
if $f'(x)=0$ then $\forall x\in[a,b]$, $f$ is constant
\end{enumerate}
\subsubsection*{proof}
suppose $f'$ is strictly positive, let $x,y\in[a,b]$ such that $x<y$. then by mean value theorem $\exists c\in(x,y)$ such that $f'(c)=\frac{f(y)-f(x)}{y-x}$ and so $(y-x)f'(c)=f(y)-f(x)$ and so $y-x>0$ and $f'(c)\ge 0 (>0)$ so $f(y)-f(x)\ge0$ an $f(y)\ge f(x)$

\subsection*{exercise 6.2.L}
a function is convex (lies below that line segment (x,f(x) to (y,f(y))) if $f(tx+(1-t)y)\le tf(x) +(1-t)f(y)$ for all $x,y$ in $[a,b]$ and all $t\in[0,1]$
\subsection*{a)} if $f$ is differentiable and $f'$ is increasing then $f$ is convex.

define $z=tx+(1-t)y$

note that $x\le z\le y$. and there exists $c_1\in(x,z),c_2\in(z,y)$ and $f'(c_1)=\frac{f(z)-f(x)}{z-x}$ and $f'(c_2)=\frac{f(y)-f(z)}{y-z}$ and $c_1< c_2$ and so $f'(c_1)\le f'(c_2)$ and $\frac{f(z)-f(x)}{z-x}\le \frac{f(y)-f(z)}{y-z}$ and on through until $f(z)(y-z)+f(z)(z-x)\le f(y)(z-x)+f(x)(y-z)$ and sub t back in for
\begin{align*}
  f(z)(y-x)&\le f(y)[tx+(1-t)y-x]+f(x)[y-tx-(1-t)y]\\
\end{align*}
and algebra to get definition
\end{document}
