\documentclass[letterpaper]{article}

\usepackage{fullpage}
\usepackage{nopageno}
\usepackage{amsmath}
\usepackage{amssymb}
\usepackage[utf8]{inputenc}
\allowdisplaybreaks

\newcommand{\abs}[1]{\left\lvert #1 \right\rvert}

\begin{document}
\title{Notes}
\date{November 19, 2014}
\maketitle
\section*{6.1.4}
\section*{6.1.6 the chain rule}
assume that $f:[a,b]\to[c.d]$ is differentiable at $x_0\in[a,b]$ and $g:[c,d]\to\mathbb{R}$ is differentiable at the point $f(x_0)$, then $g\circ f:[a,b]\to \mathbb{R}$ is differentiable at $x_0$ and $(g\circ f)$

\subsubsection*{proof}
from 6.1.4(3) because $f$ is differentiable at $x_0$, we know the there exists a function $\varphi$ such that $\varphi$ is continuous at $x_0, \varphi'(x_0)=f'(x_0)$, and $f(x)=f(x_0)+\varphi(x)(x-x_0)$ similarly $g(y)=g(f(x_0)+\psi(y)(y-f(x_0))$ because $g$ is differentiable at $f(x_0)$ $\psi$ is continuous at $f(x_0)$ and $\psi(f(x_0)=g'(f(x_0)$

we want the same condition for $g\circ f$. $g\circ f(x)=g\circ f(x_0)+\eta  (x)(x-x_0)$ for some $\eta(x)$ continous at $x_0$ and $\eta(x_0)=(g\circ f)'(x_0)$. tat $y=f(x)$. $g(f(x))=g(f(x_0))+\psi(f(x))(f(x)-f(x_0))$ and $g(f(x))=g(f(x_0))+\psi(f(x))\varphi(x)(x-x_0)$ 

\section*{6.1.7}
\subsection*{example}
let $f(x)=\sin x$ and $f^{-1}(x)=\arcsin x$. on $[-\frac{\pi}{2},\frac{\pi}{2}]$ it is injective. on $[\frac{\pi}{2},\frac{3\pi}{2}]$ $f(x)$ is injective. the inverses are not the same functions. the derivitives though will have the same values.
\subsection*{proof}
by corollary 6.1.4 we know that $f(x)=f(x_0)+\varphi(x)(x-x_0)$ when $\varphi$ is continuous at $x_0$. we want to prove that $f^{-1}(y)=f^{-1}(f(x_0))+\psi(y)(y-f(x_0))$ with $\psi$ continuous at $f(x_0)$ an $\psi(f(x_0))=\frac{1}{f'(x_0)}$. since $f,f^{-1}$ are inverses if $y=f(x)$ then $x=f^{-1}(y)$ and let $y_0=f(x_0)\Leftrightarrow x_0=f^{-1}(y_0)$ and $y-y_0=\varphi(f^{-1}(y)(f^{-1}(y)-f^{-1}(y_0)\to f^{-1}(y)-f^{-1}(y_0)$

is $\frac{1}{\varphi(f^{-1}(y)}$ continous at $f(x_0)$? $\varphi(f^{-1}(f(x_0)))=f'(x_0)\ne 0$.

\section*{from monday}
where is $\sqrt{1-\sin x}$ differentiable?

\begin{align*}
  \lim_{h\to0}\frac{\sqrt{1-\sin(x_0+h)}-\sqrt{1-\sin x_0}}{h}
  &=\lim\frac{1-\sin(x_0+h)-(1-\sin x_0)}{h(\sqrt{1-\sin(x_0+h)}\sqrt{1-\sin x_0})}\\
  &=-\cos x_0\frac{1}{2\sqrt{1-\sin x_0}}
\end{align*}
if $\sin x_0=1$ then $\cos x_0=0$ and $\lim\frac{\sqrt{1-\sin(x_0+h)}}{h}=\lim\frac{ \sqrt{1-\sin^2(x_0+h)}}{h\sqrt{1+\sin(x_0+h)}}=\lim\frac{\sqrt{\cos^2(x_0+h)}}{h\sqrt{1+\sin(x_0+h)}}=\lim\frac{\left\lvert\cos(x_0+h)-\cos x_0\right\rvert}{h\sqrt{1+\sin(x_0+h)}}$
\end{document}
