\documentclass[letterpaper]{article}

\usepackage[utf8]{inputenc}
\usepackage{fullpage}
\usepackage{nopageno}
\usepackage{amsmath}
\usepackage{amssymb}
\allowdisplaybreaks

\newcommand{\abs}[1]{\left\lvert #1 \right\rvert}

\begin{document}
\title{Notes}
\date{January 21, 2015}
\maketitle
$m*(A\cup B)\le m*A+m*B$

\subsubsection*{we want}
if $A_i\cap A_j=\emptyset$

$m*(\bigcup_{i=1}^\infty A_i)=\sum\limits_{i=1}^\infty{m*(A_i)}$

we don't always get this (sum of parts bigger than the whole)

this is a huge problem

\subsubsection*{measureable}
a set $E$ is measurable if for any  set $A$ $m*(A)=m*A\cap E)+m*(A\cap E^C)$

if we can chop $A$ in half and the size of the pieces together is the same as the size of the pieces apart then $E$ is measurable. this gives us what we want above.

\subsection*{two facts}
\begin{enumerate}
\item
if $E$ is measurable, then so is $E^C$ -- definition is symmetric with respect to complements
\item
$E$ is measurable if and only if $m*A\ge m*(A\cap E)+m*(A\cap E^C)$ for any $A$
\subsubsection*{proof}
$A=(A\cap E)\cup(A\cap E^C)\to m*(A)\le m*(A\cap E)+m*(A\cap E^C)$ (less than comes free, only need to show the greater than part)
\end{enumerate}

$E$ measurable means that $m*A=m*(A\cap E)+m*(A\cap E^C)$ for any $A$

\begin{enumerate}
\item
if $m*(E)=0$ then $E$ is measurable ($\emptyset$, singletons, cantor set)
\subsubsection*{proof}
let $A$ be a set. $A\cap E\subseteq E\to m*(A\cap E)\le m*E=0 $ and $A\cap E^C\subset A\to m*(A\cap E^C\le m*(A)$ and so $m*(A\cap E)+m*(A\cap E^C)\le 0+m*(A)$
\end{enumerate}

\section*{intersections and unions}
\subsection*{proposition}
if $E_1,E_2$ are measurable, then so is $E_1\cup E_2$.
\subsubsection*{proof}
$m*A=m*A\cap  E_1+m*A\cap E_1^C$

$m*A=m*A\cap  E_2+m*A\cap E_2^C$

we want
$m*A\ge m*A\cap  (E_1\cup E_2)+m*A\cap (E_1\cup E_2)^C$

\begin{align*}
  A&\cap(E_1\cup E_2)\\
  (A&\cap E_1)\cup (A\cap (E_2\cap E_1^C))\\
  A&\cap(E_1\cup E_2)^C\\
  A&\cap(E_1^C\cup E_2^C)\\
  m*(A\cap E_1^C)&=m*((A\cap E_1^C)\cap E_2)+m*((A\cap E_1^C)\cap E_2^C)\\
  m*(A\cap(E_1\cup E_2))&\le m*(A\cap E_1)+m*(A\cap E_2\cap E_1^2\\
  m*(A\cap E_1^C)&-m*((A\cap E_1^C)\cap E_2)=m*((A\cap E_1^C)\cap E_2^C)\\
  m*(A\cap(E_1\cup E_2))+m*((A\cap E_1^C)\cap E_2)&\le m*(A\cap E_1)+m*(A\cap E_1^C)=m*(A)\\
\end{align*}

\subsection*{proposition}
if $E_1, E_2$ are measurable, so is $E_1\cap E_2$.

$E_1\cap E_2=(E_1^C)^C\cap(E_2^C)^C$
demorgans law says $(E_1)^C\cup E_2^C)^C$ and so $(E_1^C\cup E_2^C)$ is measurable and so on

\subsection*{propostion}
if $A$ is a set and $E_1, E_2$ are measureable and $E_1\cap E_2=\emptyset$ then $m*(A\cap(E_1\cup E_2))=m*(A\cap E_1)+m*(A\cap E_2)$

\subsubsection*{proof}
$m*A=m*A\cap E_1+m*A\cap E_1^C$

$m*A\cap(E_1\cup E_2)=m*A\cap(E_1\cup E_2)\cap E_1+m*A\cap(E_1\cup E_2)\cap E_1^C=m*A\cap E_1+m*A\cap E_2$
\end{document}
