\documentclass{article}
\usepackage{fullpage}
\usepackage{nopageno}
\usepackage{amsmath}
\allowdisplaybreaks

\newcommand{\abs}[1]{\left\lvert #1 \right\rvert}
\newcommand{\degree}{\ensuremath{^\circ}}

\begin{document}
Jon Allen

HW 12

Lesson 7 problem 3. Find general series solution for PDE and BC's.
\begin{align*}
  PDE&&&\quad u_t=u_{xx}&0&<x<1&0&<t<\infty\\
  BCs&&&\left\{
  \begin{aligned}
    &u_x(0,t)=0\\
    &u_x(1,t)=0
  \end{aligned}
  \right.&&&0&<t<\infty\\
  IC&&&\quad u(x,0)=x&0&\leq x\leq 1
\end{align*}
\begin{align*}
  u(x,t)&=X(x)T(t)&u_t=u_{xx}&=XT'=X''T\\
  \frac{XT'}{XT}&=\frac{X''T}{XT}&\frac{T'}{T}=\frac{X''}{X}&=\mu \\
  T'-\mu T&=0&X''-\mu X&=0
\end{align*}
We will just assume $\mu\leq 0$.
\begin{align*}
  \mu&=-\lambda ^2\\
  T'+\lambda ^2T&=0&
  X''+\lambda ^2X&=0\\
  \frac{\mathrm{d}}{\mathrm{d}t}\left(e^{\int{\lambda ^2\,\mathrm{d}t}}T\right)&
  =e^{\int{\lambda ^2\,\mathrm{d}t}}T'+\lambda ^2e^{\int{\lambda ^2\,\mathrm{d}t}}T&
  r^2+0r+\lambda ^2&=0\\
  e^{\int{\lambda ^2\,\mathrm{d}t}}T&
  =\int{e^{\int{\lambda ^2\,\mathrm{d}t}}\cdot 0\,\mathrm{d}t}=A&
  \frac{-0\pm\sqrt{0^2-4\lambda ^2}}{2}&=r\\
  T&=Ae^{-\lambda ^2t}&0\pm\lambda i&=r\\
  &&B\cos(\lambda x)+C\sin(\lambda x)&=X\\
  u(x,t)=XT&=e^{-\lambda ^2t}\left[A\sin(\lambda x)+B\cos(\lambda x)\right]&\lambda e^{-\lambda ^2t}\left[A\cos(\lambda x)-B\sin(\lambda x)\right]&=u_x\\
  u_x(0,t)&=\lambda e^{-\lambda ^2t}\left[A\cos(\lambda0)-B\sin(\lambda0)\right]=0
  &\lambda e^{-\lambda ^2t}\left[A\cos(\lambda)-B\sin(\lambda)\right]&=u_x(1,t)=0\\
  A\lambda e^{-\lambda ^2t}&=0\\
  A&=0&-B\lambda e^{-\lambda ^2t}\sin(\lambda )&=0\\
  &&\sin(\lambda) &=0\\
  \lambda_n&=n\pi &
  u(x,t)=\sum\limits_{n=1}^\infty&{a_ne^{-{\lambda_n}^2t}\cos(\lambda_n x)}
\end{align*}
\end{document}
