\documentclass{article}
\usepackage{fullpage}
\usepackage{nopageno}
\usepackage{amsmath}
\usepackage{graphicx}
\usepackage{enumerate}
\allowdisplaybreaks

\newcommand{\abs}[1]{\left\lvert #1 \right\rvert}
\newcommand{\degree}{\ensuremath{^\circ}}

\begin{document}
Jon Allen

HW 22

Given $F(s)=\frac{1}{1+\sqrt{s}}$
\begin{enumerate}[(a)]
\item
Find $f(t)$ by expanding $F(s)$ in reciprocal powers and inverting termwise.

\begin{align*}
  \mathcal{L}^-1\{F(s)\}&=\mathcal{L}^-1\left\{\frac{1}{1+\sqrt{s}}\right\}\\
  &=\mathcal{L}^-1\left\{\sum\limits_{n=0}^\infty{(-1)^ns^{n/2}}\right\}\\
  &=\sum\limits_{n=0}^\infty{(-1)^n\mathcal{L}^-1\left\{s^{n/2}\right\}}\\
  \mathcal{L}^{-1}\{s^n\}&=\frac{t^{-n-1}}{\Gamma(-n)}\\
  &=\sum\limits_{n=0}^\infty{(-1)^n\frac{t^{-n/2-1}}{\Gamma(-n/2)}}\\
\end{align*}
\item
Reduce all occurrences of the gamma function to ordinary factorials
\begin{align*}
  &=\sum\limits_{n=0}^\infty{(-1)^n\frac{t^{-n/2-1}}{(-1-n/2)!}}\quad\text{used computer to get this}\\
\end{align*}
This result isn't really sane, but it seems to be closest to what you are looking for. I also have this, but it's not right either I think.
\begin{align*}
  &=\mathcal{L}^-1\left\{\frac{1-\sqrt{s}}{1-s}\right\}\\
  &=e^t-\mathcal{L}^-1\left\{\frac{\sqrt{s}}{1-s}\right\}\\
  &=e^t+\frac{1}{2}\mathcal{L}^-1\left\{\frac{1}{\sqrt{s}+1}\right\}+\frac{1}{2}\mathcal{L}^-1\left\{\frac{1}{\sqrt{s}-1}\right\}\\
  \frac{1}{2}\mathcal{L}^-1\left\{\frac{1}{1+\sqrt{s}}\right\}&=e^t+\frac{1}{2}\mathcal{L}^-1\left\{\frac{1}{\sqrt{s}-1}\right\}\\
  \mathcal{L}^-1\left\{\frac{1}{1+\sqrt{s}}\right\}&=2e^t+\mathcal{L}^-1\left\{\frac{\sqrt{s}+1}{s-1}\right\}\\
  &=2e^t+e^t+\mathcal{L}^-1\left\{\frac{\sqrt{s}}{s-1}\right\}\\
  &=2e^t+e^t+\frac{1}{2}\mathcal{L}^-1\left\{\frac{1}{\sqrt{s}+1}\right\}+\frac{1}{2}\mathcal{L}^-1\left\{\frac{1}{\sqrt{s}-1}\right\}\\
  &=4e^t+2e^t+\mathcal{L}^-1\left\{\frac{\sqrt{s}+1}{s-1}\right\}\\
  f(t)&=\sum\limits_{n=1}^\infty{2^ne^t}
\end{align*}
\end{enumerate}
\end{document}
