\documentclass{article}
\usepackage{fullpage}
\usepackage{nopageno}
\usepackage{amsmath}
\usepackage{graphicx}
\usepackage{enumerate}
\allowdisplaybreaks

\newcommand{\abs}[1]{\left\lvert #1 \right\rvert}
\newcommand{\degree}{\ensuremath{^\circ}}

\begin{document}
Jon Allen

HW 24

Match the usual transform table result $f(t)=\frac{1}{\sqrt{\pi t}}-e^t\text{erfc}\left(\sqrt{t}\right)$
\begin{align*}
  g(t)&=e^tc_1-e^{t}\text{erfc}(\sqrt{t})-1\\
  g(t)&=\int_0^t{f(u)\,\mathrm{d}u}\\
  f(t)&=\frac{1}{\sqrt{\pi t}}-e^t\text{erfc}\left(\sqrt{t}\right)\\
  g(t)&=\int_0^t{\frac{1}{\sqrt{\pi u}}-e^u\text{erfc}\left(\sqrt{u}\right)\,\mathrm{d}u}\\
  &=\left\lvert\frac{\ln u}{\sqrt{\pi}}-e^u\text{erfc}(\sqrt{u})+2\frac{\sqrt{u}}{\sqrt{\pi}}\right\rvert_0^t\quad\text{used maxima to integrate the second term}\\
  &=\frac{\ln t}{\sqrt{\pi}}-e^t\text{erfc}(\sqrt{t})+2\frac{\sqrt{t}}{\sqrt{\pi}}-\frac{\ln 0}{\sqrt{\pi}}+e^0\text{erfc}(\sqrt{0})
\end{align*}
\end{document}
