\documentclass{article}
\usepackage{fullpage}
\usepackage{nopageno}
\usepackage{amsmath}
\allowdisplaybreaks

\newcommand{\abs}[1]{\left\lvert #1 \right\rvert}
\newcommand{\degree}{\ensuremath{^\circ}}

\begin{document}
Jon Allen

HW 07

\begin{align*}
  u(x,t)&=\sum\limits_{n=1}^\infty{A_ne^{-(n\pi\alpha)^2t}\sin(n\pi x)}\\
  A_n&=\frac{2}{n\pi}(1-(-1)^n)\\
  u(x,t)&=\sum\limits_{n=1}^\infty{\frac{4}{(2n-1)\pi}e^{-((2n-1)\pi\alpha)^2t}\sin((2n-1)\pi x)}
\end{align*}

This seems a little simple, but all the work was really already done in HW 06.
\end{document}
