\documentclass{article}
\usepackage{fullpage}
\usepackage{nopageno}
\usepackage{amsmath}
\usepackage{graphicx}
\usepackage{enumerate}
\allowdisplaybreaks

\newcommand{\abs}[1]{\left\lvert #1 \right\rvert}
\newcommand{\degree}{\ensuremath{^\circ}}

\begin{document}
Jon Allen

HW 20

CASE 1. $\alpha_2\beta_1-\alpha_1\beta_2+\beta_1\beta_2\ne0$

Given the problem:
\begin{align*}
  \text{PDE}&&\frac{\partial u}{\partial t}&=\frac{\partial ^2u}{\partial x^2}+f(x,t)&0<&x<1,&0<&t<\infty\\
  \text{BC}&&g_1(t)&=\alpha_1\frac{\partial u}{\partial x}(0,t)+\beta_1u(0,t)&&&0<&t<\infty\\
  &&g_2(t)&=\alpha_2\frac{\partial u}{\partial x}(1,t)+\beta_2u(1,t)&{\alpha_1}^2&+{\beta_1}^2\ne0&{\alpha_2}^2&+{\beta_2}^2\ne0\\
  \text{IC}&&u(x,0)&=\phi(x)&0<&x<1
\end{align*}
Introduce the change of variables
\begin{itemize}
\item
$u(x,t)=w(x,t)+a(t)x+b(t)(1-x)$
\end{itemize}
where $a(t), b(t)$ are to be determined so that $w(x,t)$ satisfies the homogeneous BC:
\begin{align*}
  \text{BC}&&\alpha_1\frac{\partial w}{\partial x}(0,t)+\beta_1w(0,t)&=0&0<&t<\infty\\
  &&\alpha_2\frac{\partial w}{\partial x}(1,t)+\beta_2w(1,t)&=0
\end{align*}
\begin{enumerate}[(a)]
\item
Assuming $a(t), b(t)$ can be found so that $w(x,t)$ satisfies homogeneous BC, give the resulting PDE and IC for $w(x,t)$. (State it in terms of $a(t),b(t)$ - solving for them is done next.)
\begin{align*}
  \text{PDE}&&\frac{\partial u}{\partial t}&=\frac{\partial ^2u}{\partial x^2}+f(x,t)&0<&x<1,&0<&t<\infty\\
  &&\frac{\partial }{\partial t}\left(w(x,t)+a(t)x+b(t)(1-x)\right)&=\frac{\partial ^2}{\partial x^2}\left(w(x,t)+a(t)x+b(t)(1-x)\right)+f(x,t)\\
  &&\frac{\partial w}{\partial t}+x\frac{\mathrm{d} a}{\mathrm{d} t}+(1-x)\frac{\mathrm{d} b}{\mathrm{d} t}&=\frac{\partial ^2w}{\partial x^2}+\underbrace{\frac{\partial ^2}{\partial x^2}(a(t)x)}_{\to 0}+\underbrace{\frac{\partial ^2}{\partial x^2}(b(t)(1-x))}_{\to 0}+f(x,t)\\
  &&\frac{\partial w}{\partial t}+x\frac{\mathrm{d} a}{\mathrm{d} t}+(1-x)\frac{\mathrm{d} b}{\mathrm{d} t}&=\frac{\partial ^2w}{\partial x^2}+f(x,t)\\
  \text{IC}&&u(x,0)&=\phi(x)&0<&x<1\\
  &&\phi(x)&=w(x,0)+a(0)x+b(0)(1-x)
\end{align*}
\item
Show that homogeneous BC for $w(x,t)$ can be achieved (that is, a solution for $a(t),b(t)$ can be found) for \emph{arbitrary} functions $g_1(t),g_2(t)$ in the original problem if and only if $\alpha_2\beta_1-\alpha_1\beta_2+\beta_1\beta_2\ne0$
\begin{align*}
  g_1(t)&=\alpha_1\frac{\partial u}{\partial x}(0,t)+\beta_1u(0,t)\\
  g_2(t)&=\alpha_2\frac{\partial u}{\partial x}(1,t)+\beta_2u(1,t)\\
  g_1(t)&=\alpha_1\frac{\partial}{\partial x}\left(w(0,t)+a(t)\cdot0+b(t)(1-0)\right)+\beta_1\left(w(0,t)+a(t)\cdot0+b(t)(1-0)\right)\\
  &=\alpha_1\frac{\partial w}{\partial x}(0,t)+\beta_1w(0,t)+\beta_1b(t)\\
  g_1(t)-\beta_1b(t)&=\alpha_1\frac{\partial w}{\partial x}(0,t)+\beta_1w(0,t)=0\\
  g_2(t)&=\alpha_2\frac{\partial}{\partial x}\left(w(1,t)+a(t)\cdot1+b(t)(1-1)\right)+\beta_2\left(w(1,t)+a(t)\cdot1+b(t)(1-1)\right)\\
  &=\alpha_2\frac{\partial w}{\partial x}(1,t)+\beta_2w(1,t)+\beta_2a(t)\\
  g_2(t)-\beta_2a(t)&=\alpha_2\frac{\partial w}{\partial x}(1,t)+\beta_2w(1,t)=0\\
\end{align*}
\item
Assuming $\alpha_2\beta_1-\alpha_1\beta_2+\beta_1\beta_2\ne0$, give the solution for $a(t),b(t)$ in terms of $g_1(t),g_2(t)$.
\begin{align*}
  g_1(t)&=\beta_1b(t)\\
  \frac{1}{\beta_1}g_1(t)&=b(t)\\
  g_2(t)&=\beta_2a(t)\\
  \frac{1}{\beta_2}g_2(t)&=a(t)
\end{align*}
\end{enumerate}
\end{document}
