\documentclass{article}
\usepackage{fullpage}
\usepackage{nopageno}
\usepackage{amsmath}
\allowdisplaybreaks

\newcommand{\abs}[1]{\left\lvert #1 \right\rvert}
\newcommand{\degree}{\ensuremath{^\circ}}

\begin{document}
Jon Allen

HW 02

\begin{align*}
  u_t&=\alpha^2u_{xx}-\beta u & 0&<x<1\\
  u(0,t)&=1 & u(1,t)&=1\\
  \intertext{Setting the rate of change over time to zero}
  u_t&=0 & 0&=\alpha^2 u_{xx}-\beta u\\
  0&=\alpha^2r^2+0r+-\beta & r&=\frac{\pm\sqrt{-4\alpha^2(-\beta)}}{2\alpha^2}\\
  \intertext{Using the condition from the text that $\beta>0$}
  r&=\pm\sqrt{\frac{4\alpha^2\beta}{4\alpha^4}}=\pm\sqrt{\frac{\beta}{\alpha^2}}=\pm\frac{\sqrt{\beta}}{\alpha} &
  U(x)&=c_1e^{x\sqrt{\beta}/\alpha}+c_2e^{-x\sqrt{\beta}/\alpha}
\end{align*}
Since it is stated that heat is lost we know that the conservation condition $U'(0)=U'(L)$ will not hold. This is because the energy in the system is not conserved.
\end{document}
