\documentclass{article}
%\usepackage{fullpage}
\usepackage{nopageno}
\usepackage{amsmath}
\usepackage{amssymb}
\usepackage{graphicx}
\usepackage{color}
\usepackage{tabu}
\usepackage{longtable}
\usepackage{mathrsfs}
\usepackage{enumerate}
\usepackage[margin=1in]{geometry}
\usepackage{fancyhdr}
\pagestyle{fancy}
\lhead{Final 05}
\rhead{Jon Allen}
\allowdisplaybreaks

\newcommand{\abs}[1]{\left\lvert #1 \right\rvert}
\newcommand{\degree}{\ensuremath{^\circ}}

\begin{document}
\subsubsection*{PDE D.1}
\begin{align*}
  \text{PDE.}&&\frac{\partial w}{\partial t}&=\frac{\partial^2w}{\partial x^2}&&\text{for}&0&<x<\infty,&0&<t<\infty\\
  \text{BC.}&&w(0,t)&=1&&\text{for}&&&0&<t<\infty\\
  \text{IC.}&&w(x,0)&=0&&\text{for}&0&<x<\infty
\end{align*}

Solve PDE D.1 by Laplace transforming with respect to $t$. In particular, show that the Laplace transform of the solution $w(x,t)$ is $W(x,s)=\frac{1}{s}e^{-x\sqrt{s}}$ and then obtain the solution $w(x,t)$ (use tables).

\begin{align*}
  sW(x)-0&=\frac{\mathrm{d}^2W}{\mathrm{d}x^2}\\
  W(0)&=\mathcal{L}\{1\}=\frac{1}{s}\\
  0&=\frac{\mathrm{d}^2W}{\mathrm{d}x^2}-sW(x)\\
  0&=r^2+0r-s\\
  r&=\frac{\pm\sqrt{4s}}{2}=\pm\sqrt{s}\\
  W(x)&=c_1e^{x\sqrt{s}}+c_2e^{-x\sqrt{s}}\\
  W(0)&=c_1+c_2=\frac{1}{s}\\
  c_1=0&\quad c_2=\frac{1}{s}\\
  W(x)&=\frac{1}{s}e^{-x\sqrt{s}}\\
  \intertext{from handout}
  w(x,t)&=\text{erfc}\left(\frac{x}{2\sqrt{t}}\right)
\end{align*}
\end{document}
