\documentclass{article}
%\usepackage{fullpage}
\usepackage{nopageno}
\usepackage{amsmath}
\usepackage{amssymb}
\usepackage{graphicx}
\usepackage{color}
\usepackage{tabu}
\usepackage{longtable}
\usepackage{mathrsfs}
\usepackage{enumerate}
\usepackage[margin=1in]{geometry}
\usepackage{fancyhdr}
\pagestyle{fancy}
\lhead{Final 02}
\rhead{Jon Allen}
\allowdisplaybreaks

\newcommand{\abs}[1]{\left\lvert #1 \right\rvert}
\newcommand{\degree}{\ensuremath{^\circ}}

\begin{document}
\subsubsection*{PDE A.}
\begin{align*}
  \text{PDE.}&&\frac{\partial u}{\partial t}&=\frac{\partial^2u}{\partial x^2}&&\text{for}&0&<x<1,&0&<t<\infty\\
  \text{BC.}&&u_x(0,t)&=0=u_x(1,t)&&\text{for}&&&0&<t<\infty\\
  \text{IC.}&&u(x,0)&=f(x)&&\text{for}&0&<x<1
\end{align*}

For PDE A, determine the full solution for the general initial condition $f(x)$. State how orthogonality is used and how coefficients in the series expansion are determined using $f(x)$
\begin{align*}
  u_0(x,t)&=c_0\\
  u_n(x,t)&=c_ne^{-n^2\pi^2t}\cos(n\pi x)&n=1,2,3,\dots\\
  u(x,t)&=c_0+\sum\limits_{n=1}^\infty{c_ne^{-n\pi^2t}\cos(n\pi x)}\\
  u(x,t)&=\sum\limits_{n=0}^\infty{c_ne^{-n\pi^2t}\cos(n\pi x)}\\
  f(x)&=u(x,0)=\sum\limits_{n=0}^\infty{c_n\cos(n\pi x)}&\text{let }m\in\mathbb{Z}\\
  \int_{0}^1{f(x)\cos(m\pi x)\,\mathrm{d}x}&=\int_{0}^1{\cos(m\pi x)\sum\limits_{n=0}^\infty{c_n\cos(n\pi x)}\,\mathrm{d}x}\\
  \text{let }n&=m=0\\
  \int_{0}^1{c_0\cos(0)^2\,\mathrm{d}x}&=c_0\\
  \text{let }n&=m\ne 0\\
  \int_{0}^1{c_m\cos(m\pi x)^2\,\mathrm{d}x}&=\frac{1}{2}c_m\int_0^1{2\cos(m\pi x)^2\,\mathrm{d}x}\\
  &=\frac{1}{2}c_m\int_0^1{1+\cos(2m\pi x)\,\mathrm{d}x}\\
  &=\frac{1}{2}c_m\left\lvert x+\frac{1}{2m\pi}\sin(2m\pi x)\right\rvert_0^1\\
  &=\frac{1}{2}c_m+\frac{1}{2}c_m\frac{\sin(2m\pi)}{2m\pi}=\frac{1}{2}c_m&m\in\mathbb{Z}\to\sin(2m\pi)=0
  \intertext{and to establish orthogonality let $n\ne m$}
  \int_{0}^1{c_m\cos(n\pi x)\cos(m\pi x)\,\mathrm{d}x}&=\frac{1}{2}c_m\int_0^1{2\cos(n\pi x)\cos(m\pi x)\,\mathrm{d}x}\\
  &=\frac{1}{2}c_m\int_0^1{\cos(n\pi x-m\pi x)+\cos(n\pi x+m\pi x)\,\mathrm{d}x}\\
  &=\frac{1}{2}c_m\left[\frac{1}{(n-m)\pi x}\sin((n-m)\pi x)\right.\\
  &\qquad\quad\left.+\frac{1}{(n+m)\pi x}\sin((n+m)\pi x)\right]_0^1\\
  &=\frac{1}{2}c_m\left[\frac{1}{(n-m)\pi}\sin((n-m)\pi)\right.\\
  &\qquad\quad\left.+\frac{1}{(n+m)\pi}\sin((n+m)\pi)\right]&n-m,n+m\in\mathbb{Z}\\
  &=\frac{1}{2}c_m\cdot 0=0&\sin((m\pm n)\pi)=0\\
\end{align*}
And now we have everything we need to determine the full solution. Since we can find the coefficient to the $m$th term by multiplying $\cos(m\pi x)$ and then integrating, letting orthogonality kill off all the extra terms.
\begin{align*}
  u(x,t)&=\sum\limits_{n=0}^\infty{c_ne^{-n\pi^2t}\cos(n\pi x)}\\
  c_0&=\int_0^1{f(x)\,\mathrm{d}x}\\
  c_m&=2\int_{0}^1{f(x)\cos(m\pi x)\,\mathrm{d}x}&\text{where }m&=1,2,3,\dots
\end{align*}
\end{document}
