\documentclass{article}
%\usepackage{fullpage}
\usepackage{nopageno}
\usepackage{amsmath}
\usepackage{amssymb}
\usepackage{graphicx}
\usepackage{color}
\usepackage{tabu}
\usepackage{longtable}
\usepackage{mathrsfs}
\usepackage{enumerate}
\usepackage[margin=1in]{geometry}
\usepackage{fancyhdr}
\pagestyle{fancy}
\lhead{Final 06}
\rhead{Jon Allen}
\allowdisplaybreaks

\newcommand{\abs}[1]{\left\lvert #1 \right\rvert}
\newcommand{\degree}{\ensuremath{^\circ}}

\begin{document}
\subsubsection*{PDE D.2}
\begin{align*}
  \text{PDE.}&&\frac{\partial u}{\partial t}&=\frac{\partial^2u}{\partial x^2}&&\text{for}&0&<x<\infty,&0&<t<\infty\\
  \text{BC.}&&u(0,t)&=f(t)&&\text{for}&&&0&<t<\infty\\
  \text{IC.}&&u(x,0)&=0&&\text{for}&0&<x<\infty
\end{align*}

Apply the Laplace transform with respect to $t$ to PDE D.2 to obtain the relation $U(x,s)=sF(s)W(x,s)$, where $U(x,s)$ is the Laplace transform of the solution $u(x,t), F(s)$ is the transform of $f(t)$ and $W(x,s)$ is the transform of problem 5. Show that the result leads to the formula

\[u(x,t)=f(0)\text{erfc}\left(\frac{x}{2\sqrt{t}}\right)+t\int_0^1{\text{erfc}\left(\frac{x}{2\sqrt{t}}(1-u)^{-1/2}\right)f'(tu)\mathrm{d}u}\]

\begin{align*}
  sU(x)-0&=\frac{\mathrm{d}^2U}{\mathrm{d}^2x}\\
  U(0)&=F(s)\\
  0&=\frac{\mathrm{d}^2U}{\mathrm{d}^2x}-sU(x)\\
  U(x)&=c_1e^{x\sqrt{s}}+c_2e^{-x\sqrt{s}}\\
  U(0)&=F(s)=c_1+c_2\\
  c_1=0&\quad c_2=F(s)\\
  U(x)&=F(s)e^{-x\sqrt{s}}=\frac{s}{s}F(s)e^{-x\sqrt{s}}\\
  W(s)&=\frac{1}{s}e^{-x\sqrt{s}}\\
  U(x)&=sF(s)W(x)
\end{align*}
And now we do the reverse transform
\begin{align*}
  U(x)&=(sF(s)-f(0)+f(0))W(x)\\
  &=(sF(s)-f(0))W(x)+f(0)W(x)\\
  u(x,t)&=f(0)\text{erfc}\left(\frac{x}{2\sqrt{t}}\right)+\int_0^t{f'(u)\,\text{erfc}\left(\frac{x}{2\sqrt{(t-u)}}\right)\,\mathrm{d}u}\\
  &=f(0)\text{erfc}\left(\frac{x}{2\sqrt{t}}\right)+t\int_0^1{f'(tu)\,\text{erfc}\left(\frac{x}{2\sqrt{(t-tu)}}\right)\,\mathrm{d}u}\\
  &=f(0)\text{erfc}\left(\frac{x}{2\sqrt{t}}\right)+t\int_0^1{f'(tu)\,\text{erfc}\left(\frac{x}{2\sqrt{t}\sqrt{1-u}}\right)\,\mathrm{d}u}\\
\end{align*}
\end{document}
