\documentclass{article}
\usepackage{fullpage}
\usepackage{nopageno}
\usepackage{amsmath}
\allowdisplaybreaks

\newcommand{\abs}[1]{\left\lvert #1 \right\rvert}
\newcommand{\degree}{\ensuremath{^\circ}}

\begin{document}
Jon Allen

HW 11

Lesson 7 problem 1. Solve the IC. Explain how orthogonality is used.
\begin{align*}
  PDE&&&\quad u_t=u_{xx}&0&<x<1&0&<t<\infty\\
  BCs&&&\left\{
  \begin{aligned}
    &u(0,t)=0\\
    &u_x(1,t)=0
  \end{aligned}
  \right.&&&0&<t<\infty\\
  IC&&&\quad u(x,0)=x&0&\leq x\leq 1
\end{align*}
\begin{align*}
  \lambda_n&=\frac{2n-1}{2}\pi &
  u(x,t)&=\sum\limits_{n=1}^\infty{a_ne^{-{\lambda_n}^2t}\sin(\lambda_n x)}\\
  u(x,0)=x&=\sum\limits_{n=1}^\infty{a_n\sin(\lambda_n x)}&
  \int_0^1{\xi\sin(\lambda_m\xi)\,\mathrm{d}\xi}&=\sum\limits_{n=1}^\infty{a_n\int_0^1{\sin(\lambda_n\xi)\sin(\lambda_m\xi)\,\mathrm{d}\xi}}
\end{align*}
Because $\left\{\sin(\lambda_ix)\right\}_{0\leq i\leq n}$ are orthogonal functions we can convert the above equation into the following.
\begin{align*}
  \int_0^1{\xi\sin(\lambda_m\xi)\,\mathrm{d}\xi}&=a_m\int_0^1{\sin(\lambda_m\xi)^2\,\mathrm{d}\xi}\\
  &=a_m\cdot-\frac{\sin(2\lambda_m)-2\lambda_m}{4\lambda_m}\\
  &=a_m\frac{\lambda_m-\sin(\lambda_m)\cos(\lambda_m)}{2\lambda_m}\\
  \intertext{Recall that we discovered in HW 10 that $\cos(\lambda)=0$}
  &=\frac{a_m}{2}\\
  a_n&=2\int_0^1{\xi\sin(\lambda_n\xi)\,\mathrm{d}\xi}\\
  &=2\left[\frac{\sin(\lambda_nx)-\lambda_nx\cos(\lambda_nx)}{{\lambda_n}^2}\right]_0^1\\
  &=2\left[\frac{\sin(\lambda_n1)-\lambda_n1\cos(\lambda_n1)}{{\lambda_n}^2}-\frac{\sin(\lambda_n0)-\lambda_n0\cos(\lambda_n0)}{{\lambda_n}^2}\right]\\
  &=2\left[\frac{\sin(\lambda_n)}{{\lambda_n}^2}-\frac{0}{{\lambda_n}^2}\right]=2\left[\frac{\sin(\lambda_n)}{{\lambda_n}^2}\right]\\
  &=2\left[\frac{\sin\left(\frac{2n-1}{2}\pi\right)}{\left(\frac{2n-1}{2}\pi\right)^2}\right]\\
  &=\frac{8\sin\left(\frac{2n-1}{2}\pi\right)}{(2n-1)^2\pi^2}\\
  &=-1^{\left(n+1\right)}\frac{8}{(2n-1)^2\pi^2}\\
  u(x,t)&=\sum\limits_{n=1}^\infty{-1^{\left(n+1\right)}\frac{8}{(2n-1)^2\pi^2}e^{-{\lambda_n}^2t}\sin(\lambda_n x)}\\
  &=\sum\limits_{n=1}^\infty{-1^{\left(n+1\right)}\frac{8}{(2n-1)^2\pi^2}e^{-\left(\frac{2n-1}{2}\pi\right)^2t}\sin\left[\left(\frac{2n-1}{2}\pi\right) x\right]}\\
\end{align*}
\end{document}
