\documentclass{article}
\usepackage{fullpage}
\usepackage{nopageno}
\usepackage{amsmath}
\usepackage{graphicx}
\usepackage{enumerate}
\allowdisplaybreaks

\newcommand{\abs}[1]{\left\lvert #1 \right\rvert}
\newcommand{\degree}{\ensuremath{^\circ}}

\begin{document}
Jon Allen

HW 23

Given $F(s)=\frac{1}{1+\sqrt{s}}$
\begin{enumerate}[(a)]
\item
Introduce $G(s)=\frac{1}{s}F(s)$ and show that $sG(s)-G(s)=\frac{1}{\sqrt{s}}-\frac{1}{s}$
\begin{align*}
  sG(s)-G(s)&=G(s)(s-1)\\
  &=(s-1)\frac{1}{s}\frac{1}{1+\sqrt{s}}\\
  &=\frac{1}{s}\frac{(1+\sqrt{s})(1-\sqrt{s})}{1+\sqrt{s}}\\
  &=\frac{1}{s}-\frac{\sqrt{s}}{s}\\
  &=\frac{1}{s}-\frac{1}{\sqrt{s}}\\
\end{align*}
\item
Now obtain a first order DE for $g(t)$. You may assume $g(0)=0$, but show where this assumption is used.
\begin{align*}
  \mathcal{L}^{-1}\{sG(s)-G(s)\}&=\mathcal{L}^{-1}\left\{\frac{1}{s}-\frac{1}{\sqrt{s}}\right\}\\
  \mathcal{L}^{-1}\{sG(s)-0\}-g(t)&=1-\mathcal{L}^{-1}\left\{\frac{\sqrt{\pi}}{\sqrt{\pi}}\frac{1}{\sqrt{s}}\right\}\\
  \mathcal{L}^{-1}\{sG(s)-g(0)\}-g(t)&=1-\frac{1}{\sqrt{\pi}}\mathcal{L}^{-1}\left\{\frac{\Gamma(1/2)}{s^{1/2}}\right\}\\
  g'(t)-g(t)&=1-\frac{1}{\sqrt{\pi}}t^{-1/2}=1-\frac{1}{\sqrt{t\pi}}\\
\end{align*}
\item
Solve for $g(t)$
\begin{align*}
  \frac{\mathrm{d}}{\mathrm{d}t}\left(e^{\int{-1\,\mathrm{d}t}}g(t)\right)&=e^{-\int{\mathrm{d}t}}\left(1-\frac{1}{\sqrt{t\pi}}\right)\\
  e^{-t}g(t)&=\int{e^{-t}-\frac{e^-t}{\sqrt{t\pi}}\,\mathrm{d}t}\\
  e^{-t}g(t)&=-e^{-t}-\text{erfc}(\sqrt{t})+c_1\quad\text{used maxima here}\\
  g(t)&=-1-e^{t}\text{erfc}(\sqrt{t})+e^tc_1\\
  g(t)&=e^tc_1-e^{t}\text{erfc}(\sqrt{t})-1\\
\end{align*}
\item
The relation $G(s)=\frac{1}{s}F(s)$ implies a relation between $g(t)$ and $f(t)$. What is the relation?
\begin{align*}
  G(s)&=\frac{1}{s}F(s)\\
  \mathcal{L}^{-1}\{G(s)\}&=\mathcal{L}^{-1}\{\frac{1}{s}F(s)\}\\
  g(t)&=\int_0^t{f(u)\,\mathrm{d}u}
\end{align*}
Use it to find $f(t)$
\end{enumerate}
\end{document}
