\documentclass{article}
\usepackage{fullpage}
\usepackage{nopageno}
\usepackage{amsmath}
\begin{document}
Jon Allen

September 17 2013

Section 2.4 Problems 26, 38 Section 2.5 Problems 5, 19
\section*{2.4}
\subsection*{26}
Solve $\left(2t\sin y-2ty\sin(t^2)\right)\mathrm{d}t+\left(t^2\cos y+\cos(t^2)\right)\mathrm{d}y=0$
\begin{align*}
M(t,y)&=2t\sin y-2ty\sin(t^2) & N(t,y)&=t^2\cos y+\cos(t^2)\\
\frac{\partial M}{\partial y}&=2t\cos y-2t\sin(t^2) & \frac{\partial N}{\partial t}&=2t\cos y - 2t\sin(t^2)
\end{align*}
The equation is exact, we proceed by integrating $M$
\begin{align*}
\int{\left(2t\sin y-2ty\sin(t^2)\right)\,\mathrm{d}t}&=t^2\sin y+y\cos(t^2)+\phi(y)\\
N(x,y)&=\frac{\mathrm{d}}{\mathrm{d}y}\left(t^2\sin y+y\cos(t^2)+\phi(y)\right)\\
t^2\cos y+\cos(t^2)&=t^2\cos y+\cos(t^2)+\phi'(y)\\
\phi'(y)=0&,\; \phi(y)=k\\
t^2\sin y+y\cos(t^2) + k&=C_1,\,C=C_1-k\\
t^2\sin y+y\cos(t^2)&=C
\end{align*}
\subsection*{38}
Solve the IVP $\left(\cos^2 t-\sin^2 t+y\right)\mathrm{d}t+\left(\sec y \tan y + t\right)\mathrm{d}y=0,y(0)=0$
\begin{align*}
M(t,y)&=\cos^2 t-\sin^2 t+y & N(t,y)&=\sec y \tan y + t\\
\frac{\partial M}{\partial y}&=1 & \frac{\partial N}{\partial t}&=1\\
\end{align*}
\begin{align*}
\int{\left(\cos^2 t - \sin^2 t + y\right)\,\mathrm{d}t}&=\int{\cos^2 t\,\mathrm{d}t} - \int{\sin^2 t\,\mathrm{d}t} + ty+\phi(y)\\
&u=\cos t,\,\mathrm{d}v=\cos t\,\mathrm{d}t,\,\mathrm{d}u=-\sin t\,\mathrm{d}t,\,v=\sin t\\
&=\cos t\sin t-\int{\left(-\sin^2t\right)\,\mathrm{d}t} - \int{\sin^2 t\,\mathrm{d}t} + ty+\phi(y)\\
N(x,y)&=\frac{\mathrm{d}}{\mathrm{d}y}\left(\cos t\sin t+ty+\phi(y)\right)\\
\sec y \tan y + t&=t+\phi'(y)\\
\phi(y)&=\int{\frac{\sin y}{\cos^2 y}\,\mathrm{d}y}=\int{-u^{-2}\,\mathrm{d}u}\\
&=\frac{1}{\cos y}\\
\cos t\sin t+ty+\sec y&=C=\cos(0)\sin(0)+0\cdot0+\frac{1}{\cos(0)}=1\\
\cos t\sin t+ty+\sec y&=1
\end{align*}
\section*{2.5}
\subsection*{5}
Solve the Bernoulli equation $y'-2y=y^{-\frac{1}{2}}\cos t$
\begin{align*}
v=y^{3/2},\,y=v^{2/3}&,\,y'=\frac{2}{3}v^{-1/3}v'\\
\frac{2}{3}v^{-1/3}v'-2v^{2/3}&=v^{-1/3}\cos t\\
\frac{2}{3}v'-2v&=\cos t\\
v'-3v&=\frac{3}{2}\cos t & e^{\int{-3\,\mathrm{d}t}}=e^{-3t}\\
e^{-3t}v&=\int{\left(\frac{3}{2}e^{-3t}\cos t\right)\,\mathrm{d}t}=\frac{3}{2}\int{\left(e^{-3t}\cos t\right)\,\mathrm{d}t}\\
&=\frac{3}{2}\cdot\frac{e^{-3t}}{9+1}(-3\cos t+\sin t)+C\\
v&=\frac{3}{20}(-3\cos t+\sin t)+C\cdot e^{3t}\\
y^{3/2}&=\frac{3}{20}(-3\cos t+\sin t)+C\cdot e^{3t}\\
y^{3/2}+\frac{9}{20}\cos t-\frac{3}{20}\sin t-Ce^{3t}&=0
\end{align*}
\subsection*{19}
Solve $\left(ty-y^2\right)\mathrm{d}t+t\left(t-3y\right)\mathrm{d}y=0$
\begin{align*}
M(t,y)&=ty-y^2 & N(t,y)&=t^2-3ty\\
M(xt,xy)&=xtxy-(xy)^2=x^2(ty-y^2) & N(xt,xy)&=(xt)^2-3xtxy=x^2(t^2-3ty)\\
\end{align*}
Substitute $t=vy$ and $\mathrm{d}t=v\,\mathrm{d}y+y\,\mathrm{d}v$
\begin{align*}
(vy^2-y^2)(v\,\mathrm{d}y+y\,\mathrm{d}v)+(v^2y^2-3vy^2)\,\mathrm{d}y&=0=v^2y^2\,\mathrm{d}y+vy^3\,\mathrm{d}v-vy^2\,\mathrm{d}y-y^3\,\mathrm{d}v+v^2y^2\,\mathrm{d}y-3vy^2\,\mathrm{d}y\\
(v^2y^2-vy^2+v^2y^2-3vy^2)\,\mathrm{d}y&=(-vy^3+y^3)\,\mathrm{d}v=(2v^2y^2-4vy^2)\,\mathrm{d}y\\
\frac{1}{y}(2v^2-4v)\,\mathrm{d}y&=(1-v)\,\mathrm{d}v\\
\frac{1}{y}\,\mathrm{d}y&=-\frac{1}{2}\cdot\frac{v-1}{v^2-2v}\,\mathrm{d}v\\
\int{\frac{1}{y}\,\mathrm{d}y}&=-\frac{1}{4}\int{\frac{2v-2}{v^2-2v}\,\mathrm{d}v}\;\;u=v^2-2v,\,\mathrm{d}u=2v-2\,\mathrm{d}v\\
\ln |y|&=-\frac{1}{4}\int{\frac{1}{u}}\,\mathrm{d}u=-\frac{1}{4}\ln \left\lvert v^2-2v\right\rvert+C_0\\
e^{\ln |y|}&=e^{-\frac{1}{4}\ln \left\lvert v^2-2v\right\rvert+C_0}&C=e^{C_0}\\
y&=C\cdot(v^2-2v)^{-\frac{1}{4}}\\
y&=C\cdot\left(\frac{t^2}{y^2}-2\frac{t}{y}\right)^{-\frac{1}{4}}\\
\end{align*}
\end{document}
