\documentclass{article}
\usepackage{fullpage}
\usepackage{nopageno}
\usepackage{amsmath}
\allowdisplaybreaks

\newcommand{\abs}[1]{\left\lvert #1 \right\rvert}
\newcommand{\degree}{\ensuremath{^\circ}}

\begin{document}
Jon Allen

October 23, 2013

\section*{4.3}
only need the "form" of the particular solution for 14,20,24. Need the particular solution for 30. Don't forget we need the homogeneous solution too for form of solution.

\subsection*{\#14}
\[y''-4y'+3y=-e^{-9t}\]
\subsubsection*{solution}
\begin{align*}
	r^2-4r+3&=0=(r-3)(r-1) & r&=1,3 & y_h&=c_1e^{t}+c_2e^{3t}\\
	f(t)&=-e^{-9t} & S_p&=\{e^-9t\} & y_p&=Ae^{-9t}
\end{align*}

\subsection*{\#20}
\[y''+4y=4\cos t-\sin t\]
\subsubsection*{solution}
\begin{align*}
	r^2+4&=0 & r&=\frac{-0\pm\sqrt{0^2-4\cdot1\cdot4}}{2\cdot1}=\frac{\pm4i}{2}=\pm2i & y_h&=c_1\cos 2t+c_2\sin 2t \\
	f(t)&=4\cos t-\sin t & S&=\{\cos t,\sin t\}\cup\{\cos t,\sin t\}=\{\cos t,\sin t\} & y_p&=A\cos t+B\sin t
\end{align*}

\subsection*{\#24}
\[y''-4y'+13y=2te^{-2t}\sin 3t\]
\subsubsection*{solution}
\begin{align*}
	r^2&-4r+13=0 & r&=\frac{4\pm\sqrt{16-4\cdot1\cdot13}}{2}=2\pm3i & y_h&=e^{2t}\left(c_1\cos 3t+c_2\sin 3t\right)\\
	f(t)&=2te^{-2t}\sin 3t & S&=\left\{e^{-2t}\sin 3t,e^{-2t}\cos 3t,te^{-2t}\sin 3t,te^{-2t}\cos 3t\right\}
\end{align*}
\[y_p=Ae^{-2t}\sin 3t+Be^{-2t}\cos 3t+Cte^{-2t}\sin 3t+Dte^{-2t}\cos 3t\]

\subsection*{\#30}
find a general solution to $y''+3y'-4y=-32t^2$
\subsubsection*{solution}
\begin{align*}
	r^2+3r-4&=0=(r-1)(r+4) & r&=1,-4 & y_h&=c_1e^t+c_2e^{-4t}\\
	f(t)&=-32t^2 & y_p&=A+Bt+Ct^2 & {y_p}'&=B+2Ct \quad {y_p}''=2C
\end{align*}
\[2C+3B+6Ct-4A-4Bt-4Ct^2=(2C+3B-4A)+t(6C-4B)-4Ct^2=-32t^2\]
\begin{align*}
	-4C&=-32 & C&=8 & 6C-4B&=0 & B&=12 & 2C+3B-4A&=0 & \frac{52}{4}&=A=13
\end{align*}
\[y=c_1e^t+c_2e^{-4t}+8t^2+12t+13\]
\section*{4.4}

\subsection*{\#23}
find a general solution to $y''+6y'+9y=t^{-1}e^{-3t},t>0$
\subsubsection*{solution}
\begin{align*}
	r^2+6+9&=0=(r+3)^2 & r&=-3 & y_h&=c_1e^{-3t}+c_2te^{-3t}\\
	W&=e^{-3t}(e^{-3t}-3te^{-3t})+te^{-3t}3e^{-3t} & W&=e^{-6t} & {u_1}'&=-\frac{te^{-3t}}{te^{3t}e^{-6t}}=-1 \\
	{u_2}'&=\frac{e^{-3t}}{te^{3t}e^{-6t}}=t^{-1} & \int{{u_1}'\,\mathrm{d}t}&=-t & \int{\frac{1}{t}\,\mathrm{d}t}&=\ln{\abs{t}},t>0\rightarrow\ln t
\end{align*}
\[y=e^{-3t}\left(c_1+c_2t-t+t\ln t\right)=e^{-3t}\left(c_1+c_3t+t\ln t\right)\]

\subsection*{\#28}
find a general solution to $y''-10y'+25y=e^{5t}\ln 2t, t>0$
\subsubsection*{solution}
\begin{align*}
	r^2&-10r+25=0=(r-5)^2 & r&=5 & y_h&=c_1e^{5t}+c_2te^{5t}\\
	W&=e^{5t}\left(5te^{5t}+e^{5t}\right)-te^{5t}5e^{5t} & W&=e^{10t} & {u_1}'&=-\frac{te^{5t}e^{5t}\ln 2t}{e^{10t}}=-t\ln 2t\\
	{u_2}'&=\frac{e^{5t}e^{5t}\ln 2t}{e^{10t}}=\ln 2t & -\int{t\ln 2t\,\mathrm{d}t}&=-z_1w_1+\int{w_1\,\mathrm{d}z_1} &&
	\begin{aligned}
		z_1&=\ln 2t & \mathrm{d}w_1&=t\,\mathrm{d}t\\
		\mathrm{d}z_1&=\frac{1}{t}\mathrm{d}t & w_1&=\frac{1}{2}t^2
	\end{aligned}\\
	u_1&=-\frac{1}{2}t^2\ln 2t+\frac{1}{2}\int{t\,\mathrm{d}t} & u_1&=\frac{1}{2}t^2\left(\frac{1}{2}-\ln 2t\right) & \int{\ln 2t\,\mathrm{d}t}&=z_2w_2-\int{w_2\mathrm{d}z_2}\\
	&\begin{aligned}
		z_2&=\ln 2t & \mathrm{d}w_2&=\mathrm{d}t\\
		\mathrm{d}z_2&=\frac{1}{t}\mathrm{d}t & w_2&=t
	\end{aligned} &
	u_2&=t\ln t 2t-\int{\mathrm{d}t} & u_2&=t\ln 2t-t
\end{align*}
\begin{align*}
	y&=e^{5t}\left(c_1+c_2t+\frac{1}{2}t^2\left(\frac{1}{2}-\ln 2t\right)+t^2\ln 2t-t^2\right)\\
	y&=e^{5t}\left(c_1+c_2t+\frac{1}{2}t^2\ln 2t-\frac{3}{4}t^2\right)
\end{align*}
\end{document}
