\documentclass{article}
\usepackage{fullpage}
\usepackage{nopageno}
\usepackage{amsmath}
\allowdisplaybreaks

\newcommand{\abs}[1]{\left\lvert #1 \right\rvert}
\newcommand{\degree}{\ensuremath{^\circ}}

\begin{document}
Jon Allen

October 30, 2013

\section*{4.7}

\subsection*{\#8}
\[x^2y''-5xy'+10y=0\]
\subsubsection*{solution}
\begin{align*}
	0&=y(t)''-y(t)'-5y(t)'+10y(t)\\
	0&=r^2-6r+10\\
	r&=\frac{6\pm\sqrt{36-4\cdot10}}{2}=3\pm i\\
	y(t)&=e^{3t}\left(c_1\cos t+c_2\sin t\right)\\
	y(x)&=x^3\left(c_1\cos(\ln x)+c_2\sin(\ln x)\right)
\end{align*}

\subsection*{\#12}
\[x^2y''+7xy'+9y=0\]
\subsubsection*{solution}
\begin{align*}
	0&=y(t)''-y(t)'+7y(t)'+9y(t)\\
	r&=-3\\
	y(t)&=c_1e^{-3t}+c_2te^{-3t}\\
	y(x)&=c_1x^{-3}+c_2x^{-3}\ln x=\frac{c_1+c_2\ln x}{x^3}
\end{align*}

\subsection*{\#22}
\[x^2y''-5xy'+9y=x^3,\quad x>0\]
\subsubsection*{solution}
\begin{align*}
	e^{3t}&=y(t)''-y(t)'-5y(t)'+9y(t)\\
	0&=r^2-6r+9\\
	r&=3\\
	y_h(t)&=c_1e^{3t}+c_2te^{3t}\\
	y_p(t)&=At^2e^{3t}\\
	y_p(t)'&=3At^2e^{3t}+2Ate^{3t}\\
	y_p(t)''&=9At^2e^{3t}+6Ate^{3t}+6Ate^{3t}+2Ae^{3t}\\
	&=9At^2e^{3t}+12Ate^{3t}+2Ae^{3t}\\
	e^{3t}&=9At^2e^{3t}+12Ate^{3t}+2Ae^{3t}-6\left(3At^2e^{3t}+2Ate^{3t}\right)+9\left(At^2e^{3t}\right)\\
	1&=A\left(9t^2-18t^2+9t^2+12t-12t+2\right),\quad A=\frac{1}{2}\\
	y(t)&=c_1e^{3t}+c_2te^{3t}+\frac{1}{2}t^2e^{3t}\\
	y(x)&=x^3\left(c_1+c_2\ln x+\frac{1}{2}(\ln{x})^2\right)
\end{align*}

\subsection*{\#27}
\[x^2y''+xy'+4y=8,\quad x>0\]
\subsubsection*{solution}
\begin{align*}
	8&=y(t)''-y(t)'+y(t)'+4y(t)\\
	0&=r^2+4\\
	r&=\frac{0\pm\sqrt{0-4\cdot4}}{2}=\pm2i\\
	y_h(t)&=c_1\cos 2t+c_2\sin 2t\\
	y_p(t)&=A,\quad y_p(t)'=y_p(t)''=0\\
	8&=0+4A,\quad A=2\\
	y(t)&=c_1\cos 2t+c_2\sin 2t+2\\
	y(x)&=c_1\cos(2\ln x)+c_2\sin(2\ln x)+2
\end{align*}

\end{document}
