\documentclass{article}
\usepackage{fullpage}
\usepackage{nopageno}
\usepackage{amsmath}
\allowdisplaybreaks

\newcommand{\abs}[1]{\left\lvert #1 \right\rvert}

\begin{document}
\title{Notes}
\date{December 2, 2013}
\maketitle
\section*{final exam}
syllabus is everything done in class

8.4+8.7: unit step function and l-r-c circuit application

\section*{unit step function 8.4}
\begin{align*}
  f(t)&=0,0\leq t\leq a\\
      &=1, t>a\\
      &=U(t-a)\\
  g(t)&=1,0\leq t\leq b\\
      &=0, t>b\\
      &=U(t)-U(t-b)
\end{align*}
Take any $f(t)$ then $\mathcal{L}\{f(t-a)U(t-a)\}=e^{-at}F(s)$
\subsection*{example}
compute $\mathcal{L}\{(t-2)U(t-2)\}$
\begin{align*}
  \mathcal{L}\{(t-2)U(t-2)\}&=e^{-2t}\frac{1}{s^2}
\end{align*}
\subsection*{example}
compute the laplace transform of $\cos(t-\frac{\pi}{2})U(t-\frac{\pi}{2})$
\begin{align*}
  \mathcal{L}{\left\{\cos\left(t-\frac{\pi}{2}\right)U\left(t-\frac{\pi}{2}\right)\right\}}&=e^{-\frac{\pi}{2}t}\frac{s}{s^2+1}
\end{align*}
\subsection*{example}
\begin{align*}
  y''+9y&=\left\{
  \begin{aligned}
    1,\quad&0\leq t<\pi\\
    0,\quad&t>\pi
  \end{aligned}
  \right.,\quad y(0)=y'(0)=0\\
  &=1-U(t-\pi)\\
  \mathcal{L}\{y(t)\}&=Y(s)\\
  s^2Y(s)-sy(0)-y'(0)+9Y(s)&=\frac{1}{s}-\frac{e^{-\pi t}}{s}\\
  Y(s)(s^2+9)&=\frac{1-e^{-\pi t}}{s}\\
  Y(s)&=\frac{1}{s(s^2+9)}-\frac{e^{-\pi t}}{s(s^2+9)}\\
  \frac{1}{s(s^2+9)}&=\frac{A}{s}+\frac{Bs+c}{s^2+9}\\
  1&=A(s^2+9)+Bs^2+Cs=(A+B)s^2+Cs+9A\\
  C&=0,\quad A+B=0,\quad 1=9A\\
  A&=\frac{1}{9},\quad B=-\frac{1}{9},\quad C=0\\
  Y(s)&=\frac{1}{9s}-\frac{1}{9}\cdot\frac{s}{s^2+9}-e^{-\pi t}\left[\frac{1}{9s}-\frac{1}{9}\cdot\frac{s}{s^2+9}\right]\\
  y(t)&=\frac{1}{9}-\frac{1}{9}\cos 3t-\left(\frac{1}{9}-\frac{1}{9}\cos3(t-\pi)\right)U(t-\pi)
\end{align*}
\subsection*{example}
\begin{align*}
  \mathcal{L}^{-1}\left[\frac{e^{-\frac{\pi s}{2}}}{s^2+16}\right]\\
  F(s)&=\frac{1}{s^2+16},\quad a=\frac{\pi}{2}\\
  f(t)&=\frac{1}{4}\sin \left[4\left(t-\frac{\pi}{2}\right)\right]U\left(t-\frac{\pi}{2}\right)
\end{align*}
\subsection*{example}
\begin{align*}
  \mathcal{L}^{-1}\left[\frac{e^{-5s}}{s^5}\right]&=\frac{1}{24}(t-5)^4U(t-5)
\end{align*}
\end{document}
